Add rule to spend a token to generate extra after step

src/program_logic/later_res.v
@@ -18,6 +18,7 @@ Class later_tokG {Λ Σ} (IRISG : irisGS Λ Σ) := {
   num_laters_per_step_exp:
               ∀ n1 n2, n1 < n2 → 2 + num_laters_per_step n1 + num_laters_per_step n1 ≤ num_laters_per_step n2;
   step_count_next_mono : ∀ n1 n2, n1 < n2 → step_count_next n1 < step_count_next n2;
+  step_count_next_add : ∀ n1 n2, n1 < n2 → 10 + step_count_next n1 ≤ step_count_next n2;
 }.
 
 
@@ -39,19 +40,16 @@ Proof using LT.
   intros ?? ?%num_laters_per_step_exp. lia.
 Qed.
 
-(*
-Definition later_tok : iProp Σ :=
-  (∀ g ns κ, global_state_interp g ns κ ==∗
-             ∃ ns', ⌜ S ns' ≤ ns ⌝%nat ∗ global_state_interp g ns' κ).
-
-Definition is_later_tok Q : iProp Σ :=
-  □ (∀ g ns κ, global_state_interp g ns κ ∗ Q ==∗
-             ∃ ns', ⌜ S ns' ≤ ns ⌝%nat ∗ global_state_interp g ns' κ) ∗
-  □ (∀ g ns κ, global_state_interp g ns κ ==∗ global_state_interp g (S ns) κ ∗ Q).
-
-Definition later_tok : iProp Σ :=
-  ∃ Q, Q ∗ is_later_tok Q.
-*)
+Lemma later_tok_incrN n g ns mj D κ :
+  global_state_interp g ns mj D κ ==∗
+  global_state_interp g (n + ns) mj D κ ∗
+  Nat.iter n (λ P, later_tok ∗ P) True%I.
+Proof.
+  induction n.
+  - eauto.
+  - iIntros "Hg". iMod (IHn with "[$]") as "(Hg&$)".
+    by iMod (later_tok_incr with "[$]") as "($&$)".
+Qed.
 
 Lemma wpc_later_tok_use s E e k Φ Φc :
   language.to_val e = None →
@@ -106,6 +104,61 @@ Proof.
     { lia. }
     iFrame.
     iModIntro. by iApply "HΦc".
+Qed.
+
+Lemma wpc_later_tok_invest s E e k Φ Φc :
+  language.to_val e = None →
+  later_tok -∗
+  WPC e @ s; k; E {{ v, Nat.iter 10 (λ P, later_tok ∗ P) True%I -∗ Φ v }} {{ Φc }} -∗
+  WPC e @ s; k; E {{ Φ }} {{ Φc }}.
+Proof.
+  iIntros (Hnval) "Htok Hwp".
+  rewrite ?wpc_unfold /wpc_pre.
+  rewrite Hnval.
+  iIntros (mj).
+  iSplit.
+  - iIntros (q σ1 g1 ns D κ κs nt) "Hσ Hg HNC".
+    iMod (later_tok_decr with "[$]") as (ns' Heq) "Hg".
+    iMod (fupd2_mask_subseteq ∅ ∅) as "H"; [ set_solver+ | set_solver+ |].
+    iModIntro. simpl. iModIntro. iNext. iMod "H" as "_".
+    iDestruct ("Hwp" $! _) as "(Hwp&_)".
+    iSpecialize ("Hwp" $! _ _ _ _ _ _ _ with "Hσ Hg HNC").
+    iMod "Hwp".
+    iApply (step_fupd_extra.step_fupd2N_le (S (num_laters_per_step ns')) (num_laters_per_step ns)
+              with "[Hwp]").
+    { assert (Hlt: ns' < ns) by lia.
+      apply num_laters_per_step_lt in Hlt. lia.
+    }
+    iApply (step_fupd_extra.step_fupd2N_wand with "Hwp").
+    iNext. iIntros "($&H)".
+    iIntros. iMod ("H" with "[//]") as "(Hσ&Hg&Hwp&$)".
+    iFrame.
+    iMod (later_tok_incrN 10 with "[$]") as "(Hg&Htoks)".
+    iMod (global_state_interp_le _ ((step_count_next ns)) _ _ with "Hg") as "Hg".
+    { by apply step_count_next_add. }
+    iFrame.
+    iApply (wpc0_strong_mono with "Hwp"); try reflexivity.
+    iModIntro. iSplit.
+    * iIntros (?) "H". iModIntro. iApply "H"; eauto.
+    * iIntros "H". iModIntro. iApply "H"; eauto.
+  - iIntros (g ns D κs) "Hg HC".
+    iMod (later_tok_decr with "[$]") as (ns' Heq) "Hg".
+    iMod (fupd2_mask_subseteq ∅ ∅) as "H"; [ set_solver+ | set_solver+ |].
+    iApply (step_fupd_extra.step_fupd2N_le (S (num_laters_per_step ns')) (num_laters_per_step ns)).
+    { assert (Hlt: ns' < ns) by lia.
+      apply num_laters_per_step_lt in Hlt. lia.
+    }
+    rewrite Nat_iter_S. iModIntro. iModIntro. iNext.
+    iMod "H". iDestruct ("Hwp" $! _) as "(_&Hwp)".
+    iMod ("Hwp" with "[$] [$]") as "Hwp".
+    iModIntro.
+    iApply (step_fupd_extra.step_fupd2N_wand with "Hwp"). iIntros "Hwp".
+    iMod "Hwp" as "(Hg&HΦc)".
+    iMod (later_tok_incr with "[$]") as "(Hg&Htok')".
+    iMod (global_state_interp_le _ ns _ _ with "Hg") as "Hg".
+    { lia. }
+    iFrame.
+    iModIntro. eauto.
 Qed.
 
 End res.
