src/goose_lang/crash_borrow.v
@@ -34,6 +34,7 @@ Proof.
     transitivity (2 ^ 1)%nat; first by auto.
     etransitivity; last eapply (Nat.pow_le_mono_r _ 1); try (simpl; lia).
   - intros n1 n2 Hlt => /=. lia.
+  - intros n1 n2 Hlt => /=. lia.
 Qed.
 
 Lemma ownfCP_inf_le1 γ (q : Qp) (E : coPset) :
